Added big step evaluation

01Expression/01BigStep/BigStepEvaluate.thy
@@ -2,117 +2,136 @@ theory BigStepEvaluate
 imports "../Typecheck"
 begin
 
-(*
+inductive reduce :: "expr \<Rightarrow> expr \<Rightarrow> bool" (infix "\<Down>" 60) where
+  red_var [simp]: "Var x \<Down> Var x" 
+| red_abs [simp]: "Abs t e \<Down> Abs t e"
+| red_app [simp]: "e\<^sub>1 \<Down> Abs t e\<^sub>1' \<Longrightarrow> Let e\<^sub>2 e\<^sub>1' \<Down> v \<Longrightarrow> App e\<^sub>1 e\<^sub>2 \<Down> v" 
+| red_app_let [simp]: "e\<^sub>1 \<Down> Let e\<^sub>1\<^sub>1 e\<^sub>1\<^sub>2 \<Longrightarrow> Let e\<^sub>1\<^sub>1 (App e\<^sub>1\<^sub>2 (incr\<^sub>e\<^sub>e 0 e\<^sub>2)) \<Down> v \<Longrightarrow> App e\<^sub>1 e\<^sub>2 \<Down> v"
+| red_let_0 [simp]: "head_var e\<^sub>2' = Some 0 \<Longrightarrow> e\<^sub>2 \<Down> e\<^sub>2' \<Longrightarrow> e\<^sub>1 \<Down> e\<^sub>1' \<Longrightarrow> 
+    Let e\<^sub>1 (subst\<^sub>e\<^sub>e 0 (incr\<^sub>e\<^sub>e 0 e\<^sub>1) e\<^sub>2) \<Down> v \<Longrightarrow> Let e\<^sub>1 e\<^sub>2 \<Down> v"
+| red_let_S [simp]: "head_var e\<^sub>2' \<noteq> Some 0 \<Longrightarrow> e\<^sub>2 \<Down> e\<^sub>2' \<Longrightarrow> Let e\<^sub>1 e\<^sub>2 \<Down> Let e\<^sub>1 e\<^sub>2'"
+| red_rec [simp]: "Rec xs \<Down> Rec xs"
+| red_proj [simp]: "lookup xs l = Some x \<Longrightarrow> e \<Down> Rec xs \<Longrightarrow> Proj e l \<Down> Var x"
+| red_proj_let [simp]: "e \<Down> Let e\<^sub>1 e\<^sub>2 \<Longrightarrow> Let e\<^sub>1 (Proj e\<^sub>2 l) \<Down> v \<Longrightarrow> Proj e l \<Down> v" 
+| red_inj [simp]: "Inj l ts x \<Down> Inj l ts x"
+| red_case [simp]: "lookup cs l = Some e' \<Longrightarrow> e \<Down> Inj l ts x \<Longrightarrow> Let (Var x) e' \<Down> v \<Longrightarrow> 
+    Case e t cs \<Down> v"
+| red_case_let [simp]: "e \<Down> Let e\<^sub>1 e\<^sub>2 \<Longrightarrow> Let e\<^sub>1 (Case e\<^sub>2 t (map (incr\<^sub>e\<^sub>e (Suc 0)) cs)) \<Down> v \<Longrightarrow> 
+    Case e t cs \<Down> v"
+| red_fold [simp]: "Fold t x \<Down> Fold t x"
+| red_unfold [simp]: "e \<Down> Fold t x \<Longrightarrow> Unfold t e \<Down> Var x"  
+| red_unfold_let [simp]: "e \<Down> Let e\<^sub>1 e\<^sub>2 \<Longrightarrow> Let e\<^sub>1 (Unfold t e\<^sub>2) \<Down> v \<Longrightarrow> Unfold t e \<Down> v" 
+| red_tyabs [simp]: "TyAbs k e \<Down> TyAbs k e"
+| red_tyapp [simp]: "e \<Down> TyAbs k e' \<Longrightarrow> subst\<^sub>t\<^sub>e 0 t e' \<Down> v \<Longrightarrow> TyApp e t \<Down> v" 
+| red_tyapp_let [simp]: "e \<Down> Let e\<^sub>1 e\<^sub>2 \<Longrightarrow> Let e\<^sub>1 (TyApp e\<^sub>2 t) \<Down> v \<Longrightarrow> TyApp e t \<Down> v" 
+| red_tylet [simp]: "subst\<^sub>t\<^sub>e 0 t e \<Down> v \<Longrightarrow> TyLet t e \<Down> v" 
 
-inductive evaluate :: "expr \<Rightarrow> expr \<Rightarrow> bool" (infix "\<leadsto>" 60) where
-  ev_app1 [simp]: "e\<^sub>1 \<leadsto> e\<^sub>1' \<Longrightarrow> App e\<^sub>1 e\<^sub>2 \<leadsto> App e\<^sub>1' e\<^sub>2" 
-| ev_app2 [simp]: "App (Abs t e\<^sub>1) e\<^sub>2 \<leadsto> Let e\<^sub>2 e\<^sub>1"
-| ev_app_let [simp]: "is_value e\<^sub>1\<^sub>2 \<Longrightarrow> App (Let e\<^sub>1\<^sub>1 e\<^sub>1\<^sub>2) e\<^sub>2 \<leadsto> Let e\<^sub>1\<^sub>1 (App e\<^sub>1\<^sub>2 (incr\<^sub>e\<^sub>e 0 e\<^sub>2))"
-| ev_let1 [simp]: "e\<^sub>2 \<leadsto> e\<^sub>2' \<Longrightarrow> Let e\<^sub>1 e\<^sub>2 \<leadsto> Let e\<^sub>1 e\<^sub>2'"
-| ev_let2 [simp]: "e\<^sub>1 \<leadsto> e\<^sub>1' \<Longrightarrow> head_var e\<^sub>2 = Some 0 \<Longrightarrow> Let e\<^sub>1 e\<^sub>2 \<leadsto> Let e\<^sub>1' e\<^sub>2"
-| ev_let3 [simp]: "is_value e\<^sub>1 \<Longrightarrow> head_var e\<^sub>2 = Some 0 \<Longrightarrow> 
-    Let e\<^sub>1 e\<^sub>2 \<leadsto> Let e\<^sub>1 (subst\<^sub>e\<^sub>e 0 (incr\<^sub>e\<^sub>e 0 e\<^sub>1) e\<^sub>2)"
-| ev_proj1 [simp]: "e \<leadsto> e' \<Longrightarrow> Proj e l \<leadsto> Proj e' l"
-| ev_proj2 [simp]: "lookup fs l = Some x \<Longrightarrow> Proj (Rec fs) l \<leadsto> Var x" 
-| ev_proj_let [simp]: "is_value e\<^sub>2 \<Longrightarrow> Proj (Let e\<^sub>1 e\<^sub>2) l \<leadsto> Let e\<^sub>1 (Proj e\<^sub>2 l)" 
-| ev_case1 [simp]: "e \<leadsto> e' \<Longrightarrow> Case e t cs \<leadsto> Case e' t cs"
-| ev_case2 [simp]: "lookup cs l = Some e \<Longrightarrow> Case (Inj l ts x) t cs \<leadsto> Let (Var x) e"
-| ev_case_let [simp]: "is_value e\<^sub>2 \<Longrightarrow> 
-    Case (Let e\<^sub>1 e\<^sub>2) t cs \<leadsto> Let e\<^sub>1 (Case e\<^sub>2 t (map (incr\<^sub>e\<^sub>e (Suc 0)) cs))" 
-| ev_unfold1 [simp]: "e \<leadsto> e' \<Longrightarrow> Unfold t e \<leadsto> Unfold t e'"  
-| ev_unfold2 [simp]: "Unfold t (Fold t e) \<leadsto> Var e" 
-| ev_unfold_let [simp]: "is_value e\<^sub>2 \<Longrightarrow> Unfold t (Let e\<^sub>1 e\<^sub>2) \<leadsto> Let e\<^sub>1 (Unfold t e\<^sub>2)" 
-| ev_tyapp1 [simp]: "e \<leadsto> e' \<Longrightarrow> TyApp e t \<leadsto> TyApp e' t" 
-| ev_tyapp2 [simp]: "TyApp (TyAbs k e) t \<leadsto> subst\<^sub>t\<^sub>e 0 t e" 
-| ev_tyapp_let [simp]: "is_value e\<^sub>2 \<Longrightarrow> TyApp (Let e\<^sub>1 e\<^sub>2) t \<leadsto> Let e\<^sub>1 (TyApp e\<^sub>2 t)" 
-| ev_tylet [simp]: "TyLet t e \<leadsto> subst\<^sub>t\<^sub>e 0 t e" 
-
-lemma canonical_arrow [simp]: "\<Delta>,\<Gamma> \<turnstile> e : Arrow t\<^sub>1 t\<^sub>2 \<Longrightarrow> is_value e \<Longrightarrow> 
-    (\<exists>e'. e = Abs t\<^sub>1 e') \<or> (\<exists>e\<^sub>1 e\<^sub>2. e = Let e\<^sub>1 e\<^sub>2 \<and> is_value e\<^sub>2)"
-  by (induction \<Gamma> e "Arrow t\<^sub>1 t\<^sub>2" rule: typecheck_typecheck_cs.inducts(1)) simp_all
-
-lemma canonical_record [simp]: "\<Delta>,\<Gamma> \<turnstile> e : Record ts \<Longrightarrow> is_value e \<Longrightarrow> 
-    (\<exists>fs. e = Rec fs \<and> \<Delta>,\<Gamma> \<turnstile>\<^sub>x\<^sub>s fs : ts) \<or> (\<exists>e\<^sub>1 e\<^sub>2. e = Let e\<^sub>1 e\<^sub>2 \<and> is_value e\<^sub>2)"
-  by (induction \<Gamma> e "Record ts" rule: typecheck_typecheck_cs.inducts(1)) simp_all
-
-lemma canonical_variant [simp]: "\<Delta>,\<Gamma> \<turnstile> e : Variant ts \<Longrightarrow> is_value e \<Longrightarrow> 
-    (\<exists>l e'. e = Inj l ts e' \<and> l < length ts) \<or> (\<exists>e\<^sub>1 e\<^sub>2. e = Let e\<^sub>1 e\<^sub>2 \<and> is_value e\<^sub>2)"
-  by (induction \<Gamma> e "Variant ts" rule: typecheck_typecheck_cs.inducts(1)) auto
-
-lemma canonical_inductive [simp]: "\<Delta>,\<Gamma> \<turnstile> e : Inductive k t \<Longrightarrow> is_value e \<Longrightarrow> 
-    (\<exists>e'. e = Fold t e') \<or> (\<exists>e\<^sub>1 e\<^sub>2. e = Let e\<^sub>1 e\<^sub>2 \<and> is_value e\<^sub>2)"
-  by (induction \<Gamma> e "Inductive k t" rule: typecheck_typecheck_cs.inducts(1)) auto
-
-lemma canonical_forall [simp]: "\<Delta>,\<Gamma> \<turnstile> e : Forall k t \<Longrightarrow> is_value e \<Longrightarrow> 
-    (\<exists>e'. e = TyAbs k e') \<or> (\<exists>e\<^sub>1 e\<^sub>2. e = Let e\<^sub>1 e\<^sub>2 \<and> is_value e\<^sub>2)"
-  by (induction \<Gamma> e "Forall k t" rule: typecheck_typecheck_cs.inducts(1)) auto
-
-lemma lookup_in_tc [simp]: "\<Delta>,\<Gamma> \<turnstile>\<^sub>x\<^sub>s fs : ts \<Longrightarrow> lookup ts l = Some t \<Longrightarrow> \<exists>e. lookup fs l = Some e"
-  by (induction fs l arbitrary: ts rule: lookup.induct) auto
-
-lemma progress': "\<Delta>,\<Gamma> \<turnstile> e : t \<Longrightarrow> 
-  is_value e \<or> (\<exists>e'. e \<leadsto> e') \<or> (\<exists>x < length \<Gamma>. head_var e = Some x)"
-    and "\<Delta>,\<Gamma> \<turnstile>\<^sub>c cs : ts \<rightarrow> t \<Longrightarrow> l < length ts \<Longrightarrow> \<exists>c. lookup cs l = Some c"
-  proof (induction \<Delta> \<Gamma> e t and \<Delta> \<Gamma> cs ts t arbitrary: and l rule: typecheck_typecheck_cs.inducts)
-  case tc_var
-    thus ?case by (metis lookup_less_than head_var.simps(1))
-  next case tc_app
-    thus ?case by (metis canonical_arrow ev_app1 ev_app2 ev_app_let head_var.simps(3))
-  next case (tc_let \<Delta> \<Gamma> e\<^sub>1 t\<^sub>1 e\<^sub>2 t\<^sub>2)
-    thus ?case
-      proof (cases "is_value e\<^sub>2")
-      case False note F = False
-        thus ?thesis
-          proof (cases "\<exists>e\<^sub>2'. e\<^sub>2 \<leadsto> e\<^sub>2'")
-          case False
-            with tc_let F obtain x where X: "x < Suc (length \<Gamma>) \<and> head_var e\<^sub>2 = Some x" by fastforce
-            thus ?thesis 
-              proof (cases x)
-              case 0
-                with X show ?thesis
-                  proof (cases "is_value e\<^sub>1")
-                  case False
-                    with tc_let X 0 ev_let2 show ?thesis by fastforce
-                  qed (metis ev_let3)
-              qed simp_all
-          qed (metis ev_let1)
-      qed simp_all
-  next case tc_proj
-    thus ?case 
-      by (metis canonical_record ev_proj1 ev_proj2 ev_proj_let lookup_in_tc head_var.simps(6))
-  next case tc_case
-    thus ?case by (metis canonical_variant ev_case1 ev_case2 ev_case_let head_var.simps(8))
-  next case tc_unfold
-    thus ?case by (metis canonical_inductive ev_unfold1 ev_unfold2 ev_unfold_let head_var.simps(10))
-  next case tc_tyapp
-    thus ?case by simp (metis canonical_forall ev_tyapp1 ev_tyapp2 ev_tyapp_let)
-  next case tc_tylet
-    thus ?case by (metis ev_tylet)
-  next case tcc_cons
-    thus ?case by (induction l) simp_all
-  qed simp_all
-
-theorem progress: "\<Delta>,[] \<turnstile> e : t \<Longrightarrow> is_value e \<or> (\<exists>e'. e \<leadsto> e')"
-  using progress' by fastforce
-
-theorem preservation: "e \<leadsto> e' \<Longrightarrow> \<Delta>,\<Gamma> \<turnstile> e : t \<Longrightarrow> \<Delta>,\<Gamma> \<turnstile> e' : t"
-  proof (induction e e' arbitrary: \<Delta> \<Gamma> t rule: evaluate.induct) 
-  case (ev_proj2 l xs x)
+theorem preservation [elim]: "e \<Down> v \<Longrightarrow> \<Delta>,\<Gamma> \<turnstile> e : t \<Longrightarrow> \<Delta>,\<Gamma> \<turnstile> v : t"
+  proof (induction e v arbitrary: \<Gamma> t rule: reduce.induct) 
+  case (red_proj xs l x e)
     hence "lookup \<Gamma> x = Some t" by fastforce
     thus ?case by simp
-  next case (ev_case2 cs l e ts x t')
-    then obtain tt where "(lookup \<Gamma> x = Some tt) \<and> lookup ts l = Some tt \<and> 
-      (\<forall>tt \<in> set ts. \<Delta> \<turnstile>\<^sub>k tt : Star) \<and> (\<Delta>,\<Gamma> \<turnstile>\<^sub>c cs : ts \<rightarrow> t') \<and> t' = t" by fastforce
-    moreover with ev_case2 have "\<Delta>,insert_at 0 tt \<Gamma> \<turnstile> e : t" by fastforce
-    ultimately show ?case by (metis tc_let tc_var)
-  next case (ev_tyapp2 k e t')
-    then obtain tt where T: "(insert_at 0 k \<Delta>,map (incr\<^sub>t\<^sub>t 0) \<Gamma> \<turnstile> e : tt) \<and> (\<Delta> \<turnstile>\<^sub>k t' : k) \<and> 
-      t = subst\<^sub>t\<^sub>t 0 t' tt" by fastforce
-    moreover hence "\<Delta>,map (subst\<^sub>t\<^sub>t 0 t') (map (incr\<^sub>t\<^sub>t 0) \<Gamma>) \<turnstile> subst\<^sub>t\<^sub>e 0 t' e : subst\<^sub>t\<^sub>t 0 t' tt" 
-      using tc_subst\<^sub>t\<^sub>e by fastforce
-    ultimately show ?case by simp
+  next case (red_case cs l e' e ts x v tt)
+    moreover hence "(\<Delta>,\<Gamma> \<turnstile> e : Variant ts) \<and> (\<Delta>,\<Gamma> \<turnstile>\<^sub>c cs : ts \<rightarrow> t) \<and> (\<Delta> \<turnstile>\<^sub>k t : Star)" by fastforce
+    moreover with red_case obtain t' where T: "lookup \<Gamma> x = Some t' \<and> lookup ts l = Some t' \<and> 
+      (\<forall>tt \<in> set ts. \<Delta> \<turnstile>\<^sub>k tt : Star)" by blast
+    ultimately have "\<Delta>,insert_at 0 t' \<Gamma> \<turnstile> e' : t" by auto
+    with red_case T show ?case by (metis tc_let tc_var)
+  next case (red_tyapp e k e' tt v)
+    then obtain t' k' where T: "t = subst\<^sub>t\<^sub>t 0 tt t' \<and> (\<Delta>,\<Gamma> \<turnstile> e : Forall k' t') \<and> (\<Delta> \<turnstile>\<^sub>k tt : k')" 
+      by fastforce
+    with red_tyapp have "insert_at 0 k' \<Delta>,map (incr\<^sub>t\<^sub>t 0) \<Gamma> \<turnstile> e' : t'" by fastforce
+    with T have "\<Delta>,map (subst\<^sub>t\<^sub>t 0 tt) (map (incr\<^sub>t\<^sub>t 0) \<Gamma>) \<turnstile> subst\<^sub>t\<^sub>e 0 tt e' : subst\<^sub>t\<^sub>t 0 tt t'" 
+      by (metis tc_subst\<^sub>t\<^sub>e le0)
+    with red_tyapp T show ?case by simp
   qed fastforce+
 
-*)
+(* we can't actually do progress because the language is not normalizing *)
+(* instead we prove the weaker claim that we get a value _if it's defined at all_ *)
+
+lemma reduce_to_value' [simp]: "e \<Down> v \<Longrightarrow> \<Delta>,\<Gamma> \<turnstile> e : t \<Longrightarrow> 
+      is_value v \<or> (\<exists>x < length \<Gamma>. head_var v = Some x)"
+  proof (induction e v arbitrary: \<Gamma> rule: reduce.induct)
+  case (red_app e\<^sub>1 tt e\<^sub>1' e\<^sub>2 v)
+    then obtain t\<^sub>1 where T: "(\<Delta>,\<Gamma> \<turnstile> e\<^sub>1 : Arrow t\<^sub>1 t) \<and> (\<Delta>,\<Gamma> \<turnstile> e\<^sub>2 : t\<^sub>1)" by fastforce
+    with red_app have "\<Delta>,\<Gamma> \<turnstile> Abs tt e\<^sub>1' : Arrow t\<^sub>1 t" by fastforce
+    with T have "\<Delta>,\<Gamma> \<turnstile> Let e\<^sub>2 e\<^sub>1' : t" by auto
+    with red_app show ?case by simp
+  next case (red_app_let e\<^sub>1 e\<^sub>1\<^sub>1 e\<^sub>1\<^sub>2 e\<^sub>2 v)
+    then obtain t\<^sub>1 where T: "(\<Delta>,\<Gamma> \<turnstile> e\<^sub>1 : Arrow t\<^sub>1 t) \<and> (\<Delta>,\<Gamma> \<turnstile> e\<^sub>2 : t\<^sub>1)" by fastforce
+    with red_app_let have "\<Delta>,\<Gamma> \<turnstile> Let e\<^sub>1\<^sub>1 e\<^sub>1\<^sub>2 : Arrow t\<^sub>1 t" by fastforce
+    then obtain tt where "(\<Delta>,\<Gamma> \<turnstile> e\<^sub>1\<^sub>1 : tt) \<and> (\<Delta>,insert_at 0 tt \<Gamma> \<turnstile> e\<^sub>1\<^sub>2 : Arrow t\<^sub>1 t)" by fastforce
+    with T have "\<Delta>,\<Gamma> \<turnstile> Let e\<^sub>1\<^sub>1 (App e\<^sub>1\<^sub>2 (incr\<^sub>e\<^sub>e 0 e\<^sub>2)) : t" by fastforce
+    with red_app_let show ?case by simp
+  next case (red_let_0 e\<^sub>2' e\<^sub>2 e\<^sub>1 e\<^sub>1' v)
+    hence "\<Delta>,\<Gamma> \<turnstile> Let e\<^sub>1 (subst\<^sub>e\<^sub>e 0 (incr\<^sub>e\<^sub>e 0 e\<^sub>1) e\<^sub>2) : t" by fastforce
+    with red_let_0 show ?case by simp
+  next case (red_let_S e\<^sub>2' e\<^sub>2 e\<^sub>1)
+    from red_let_S have "\<Delta>,\<Gamma> \<turnstile> Let e\<^sub>1 e\<^sub>2 : t" by simp
+    then obtain t\<^sub>1 where "(\<Delta>,\<Gamma> \<turnstile> e\<^sub>1 : t\<^sub>1) \<and> (\<Delta>,insert_at 0 t\<^sub>1 \<Gamma> \<turnstile> e\<^sub>2 : t)" by fastforce
+    with red_let_S have "is_value e\<^sub>2' \<or> (\<exists>x < length (insert_at 0 t\<^sub>1 \<Gamma>). head_var e\<^sub>2' = Some x)" 
+      by blast
+    with red_let_S show ?case by (auto split: nat.splits)
+  next case (red_proj xs l x e)
+    then obtain ts where "(\<Delta>,\<Gamma> \<turnstile> e : Record ts) \<and> lookup ts l = Some t" by fastforce
+    with red_proj have "\<Delta>,\<Gamma> \<turnstile> Rec xs : Record ts" by fastforce
+    with red_proj show ?case by auto
+  next case (red_proj_let e e\<^sub>1 e\<^sub>2 l v)
+    then obtain ts where T: "(\<Delta>,\<Gamma> \<turnstile> e : Record ts) \<and> lookup ts l = Some t" by fastforce
+    with red_proj_let have "\<Delta>,\<Gamma> \<turnstile> Let e\<^sub>1 e\<^sub>2 : Record ts" by fastforce
+    then obtain t\<^sub>1 where "(\<Delta>,\<Gamma> \<turnstile> e\<^sub>1 : t\<^sub>1) \<and> (\<Delta>,insert_at 0 t\<^sub>1 \<Gamma> \<turnstile> e\<^sub>2 : Record ts)" by fastforce
+    with T have "\<Delta>,\<Gamma> \<turnstile> Let e\<^sub>1 (Proj e\<^sub>2 l) : t" by fastforce
+    with red_proj_let show ?case by simp
+  next case (red_case cs l e' e ts x v tt) 
+    then obtain ts' where T: "tt = t \<and> (\<Delta>,\<Gamma> \<turnstile> e : Variant ts') \<and> (\<Delta>,\<Gamma> \<turnstile>\<^sub>c cs : ts' \<rightarrow> t) \<and> 
+      (\<Delta> \<turnstile>\<^sub>k t : Star)" by fastforce
+    with red_case have "\<Delta>,\<Gamma> \<turnstile> Inj l ts x : Variant ts'" by fastforce
+    then obtain t' where S: "ts' = ts \<and> lookup \<Gamma> x = Some t' \<and> lookup ts l = Some t' \<and> 
+      (\<forall>tt \<in> set ts. \<Delta> \<turnstile>\<^sub>k tt : Star)" by fastforce
+    with red_case T have X: "\<Delta>,insert_at 0 t' \<Gamma> \<turnstile> e' : t" by auto
+    from S have "\<Delta>,\<Gamma> \<turnstile> Var x : t'" by simp
+    with X have "\<Delta>,\<Gamma> \<turnstile> Let (Var x) e' : t" by simp
+    with red_case T show ?case by simp
+  next case (red_case_let e e\<^sub>1 e\<^sub>2 tt cs v)
+    then obtain ts where T: "t = tt \<and> (\<Delta>,\<Gamma> \<turnstile> e : Variant ts) \<and> (\<Delta>,\<Gamma> \<turnstile>\<^sub>c cs : ts \<rightarrow> t) \<and> 
+      (\<Delta> \<turnstile>\<^sub>k t : Star)" by fastforce
+    with red_case_let have "\<Delta>,\<Gamma> \<turnstile> Let e\<^sub>1 e\<^sub>2 : Variant ts" by fastforce
+    then obtain t\<^sub>1 where "(\<Delta>,\<Gamma> \<turnstile> e\<^sub>1 : t\<^sub>1) \<and> (\<Delta>,insert_at 0 t\<^sub>1 \<Gamma> \<turnstile> e\<^sub>2 : Variant ts)" by fastforce
+    with T have "\<Delta>,\<Gamma> \<turnstile> Let e\<^sub>1 (Case e\<^sub>2 tt (map (incr\<^sub>e\<^sub>e (Suc 0)) cs)) : t" by fastforce
+    with red_case_let show ?case by simp
+  next case (red_unfold e tt x) 
+    then obtain k where T: "t = subst\<^sub>t\<^sub>t 0 (Inductive k tt) tt \<and> (\<Delta>,\<Gamma> \<turnstile> e : Inductive k tt) \<and> 
+      (insert_at 0 k \<Delta> \<turnstile>\<^sub>k tt : Star)" by fastforce
+    with red_unfold have "\<Delta>,\<Gamma> \<turnstile> Fold tt x : Inductive k tt" by fastforce
+    hence "lookup \<Gamma> x = Some (subst\<^sub>t\<^sub>t 0 (Inductive k tt) tt) \<and> (insert_at 0 k \<Delta> \<turnstile>\<^sub>k tt : Star)" 
+      by fastforce
+    with T show ?case by auto
+  next case (red_unfold_let e e\<^sub>1 e\<^sub>2 tt v)
+    then obtain k where T: "t = subst\<^sub>t\<^sub>t 0 (Inductive k tt) tt \<and> (\<Delta>,\<Gamma> \<turnstile> e : Inductive k tt) \<and> 
+      (insert_at 0 k \<Delta> \<turnstile>\<^sub>k tt : Star)" by fastforce
+    with red_unfold_let have "\<Delta>,\<Gamma> \<turnstile> Let e\<^sub>1 e\<^sub>2 : Inductive k tt" by fastforce
+    then obtain t\<^sub>1 where "(\<Delta>,\<Gamma> \<turnstile> e\<^sub>1 : t\<^sub>1) \<and> (\<Delta>,insert_at 0 t\<^sub>1 \<Gamma> \<turnstile> e\<^sub>2 : Inductive k tt)" 
+      by fastforce
+    with T have "\<Delta>,\<Gamma> \<turnstile> Let e\<^sub>1 (Unfold tt e\<^sub>2) : t" by fastforce
+    with red_unfold_let show ?case by simp
+  next case (red_tyapp e k e' t' v)
+    then obtain tt kk where T: "t = subst\<^sub>t\<^sub>t 0 t' tt \<and> (\<Delta>,\<Gamma> \<turnstile> e : Forall kk tt) \<and> (\<Delta> \<turnstile>\<^sub>k t' : kk)" 
+      by fastforce
+    with red_tyapp have "\<Delta>,\<Gamma> \<turnstile> TyAbs k e' : Forall kk tt" by fastforce
+    hence "kk = k \<and> insert_at 0 k \<Delta>,map (incr\<^sub>t\<^sub>t 0) \<Gamma> \<turnstile> e' : tt" by fastforce
+    with T have "\<Delta>,map (subst\<^sub>t\<^sub>t 0 t') (map (incr\<^sub>t\<^sub>t 0) \<Gamma>) \<turnstile> subst\<^sub>t\<^sub>e 0 t' e' : subst\<^sub>t\<^sub>t 0 t' tt" 
+      by (metis tc_subst\<^sub>t\<^sub>e le0)
+    with red_tyapp T show ?case by simp
+  next case (red_tyapp_let e e\<^sub>1 e\<^sub>2 tt v) 
+    then obtain t' k where T: "t = subst\<^sub>t\<^sub>t 0 tt t' \<and> (\<Delta>,\<Gamma> \<turnstile> e : Forall k t') \<and> (\<Delta> \<turnstile>\<^sub>k tt : k)" 
+      by fastforce
+    with red_tyapp_let have "\<Delta>,\<Gamma> \<turnstile> Let e\<^sub>1 e\<^sub>2 : Forall k t'" by fastforce
+    then obtain t\<^sub>1 where "(\<Delta>,\<Gamma> \<turnstile> e\<^sub>1 : t\<^sub>1) \<and> (\<Delta>,insert_at 0 t\<^sub>1 \<Gamma> \<turnstile> e\<^sub>2 : Forall k t')" by fastforce
+    with T have "\<Delta>,\<Gamma> \<turnstile> Let e\<^sub>1 (TyApp e\<^sub>2 tt) : t" by fastforce
+    with red_tyapp_let show ?case by simp
+  qed auto
+
+theorem reduce_to_value: "e \<Down> v \<Longrightarrow> \<Delta>,[] \<turnstile> e : t \<Longrightarrow> is_value v"
+  using reduce_to_value' by fastforce
 
 end
