01Expression/01BigStep/BigStepDeterminism.thy
@@ -2,164 +2,56 @@ theory BigStepDeterminism
 imports BigStepEvaluate
 begin
 
-(*
-
-lemma [elim]: "head_var e = Some x \<Longrightarrow> is_value e \<Longrightarrow> False"
-  by (induction e arbitrary: x) (auto split: option.splits nat.splits)
-
-lemma [elim]: "e \<leadsto> e' \<Longrightarrow> is_value e \<Longrightarrow> False"
-  by (induction e e' rule: evaluate.induct) auto
-
-lemma [elim]: "e \<leadsto> e' \<Longrightarrow> head_var e = Some x \<Longrightarrow> False"
-  by (induction e e' arbitrary: x rule: evaluate.induct) (auto split: option.splits nat.splits)
-
-theorem determinism [elim]: "e \<leadsto> e' \<Longrightarrow> e \<leadsto> e'' \<Longrightarrow> e' = e''"
-  proof (induction e e' arbitrary: e'' rule: evaluate.induct)
-  case (ev_app1 e\<^sub>1 e\<^sub>1' e\<^sub>2)
-    with ev_app1(3) show ?case
-      proof (induction "App e\<^sub>1 e\<^sub>2" e'' rule: evaluate.induct)
-      case ev_app2
-        hence False by auto
-        thus ?case by simp
-      next case ev_app_let
-        hence False by auto
-        thus ?case by simp
-      qed simp_all
-  next case (ev_app2 t e\<^sub>1 e\<^sub>2)
-    thus ?case by (induction "App (Abs t e\<^sub>1) e\<^sub>2" e'' rule: evaluate.induct) auto
-  next case (ev_app_let e\<^sub>1\<^sub>2 e\<^sub>1\<^sub>1 e\<^sub>2)
-    with ev_app_let(2) show ?case
-      proof (induction "App (Let e\<^sub>1\<^sub>1 e\<^sub>1\<^sub>2) e\<^sub>2" e'' rule: evaluate.induct)
-      case ev_app1
-        hence False by auto
-        thus ?case by simp
-      qed simp_all
-  next case (ev_let1 e\<^sub>2 e\<^sub>2' e\<^sub>1)
-    with ev_let1(3) show ?case
-      proof (induction "Let e\<^sub>1 e\<^sub>2" e'' rule: evaluate.induct) 
-      case ev_let2
-        hence False by fast
-        thus ?case by simp
-      next case ev_let3
-        hence False by auto
-        thus ?case by simp
-      qed simp_all
-  next case (ev_let2 e\<^sub>1 e\<^sub>1' e\<^sub>2)
-    with ev_let2(4) show ?case
-      proof (induction "Let e\<^sub>1 e\<^sub>2" e'' rule: evaluate.induct) 
-      case ev_let1
-        hence False by fast
-        thus ?case by simp
-      next case ev_let3
-        hence False by auto
-        thus ?case by simp
-      qed simp_all
-  next case (ev_let3 e\<^sub>1 e\<^sub>2)
-    with ev_let3(3) show ?case
-      proof (induction "Let e\<^sub>1 e\<^sub>2" e'' rule: evaluate.induct) 
-      case ev_let1
-        hence False by auto
-        thus ?case by simp
-      next case ev_let2
-        hence False by auto
-        thus ?case by simp
-      qed simp_all
-  next case (ev_proj1 e e' l)
-    with ev_proj1(3) show ?case
-      proof (induction "Proj e l" e'' rule: evaluate.induct)
-      case ev_proj2
-        hence False by auto
-        thus ?case by simp
-      next case ev_proj_let
-        hence False by auto
-        thus ?case by simp
-      qed simp_all
-  next case (ev_proj2 fs l e)
-    with ev_proj2(2) show ?case
-      proof (induction "Proj (Rec fs) l" e'' rule: evaluate.induct)
-      case ev_proj1
-        hence False by auto
-        thus ?case by simp
-      qed simp_all
-  next case (ev_proj_let e\<^sub>2 e\<^sub>1 l)
-    with ev_proj_let(2) show ?case
-      proof (induction "Proj (expr.Let e\<^sub>1 e\<^sub>2) l" e'' rule: evaluate.induct)
-      case ev_proj1
-        hence False by auto
-        thus ?case by simp
-      qed simp_all
-  next case (ev_case1 e e' t cs)
-    with ev_case1(3) show ?case
-      proof (induction "Case e t cs" e'' rule: evaluate.induct)
-      case ev_case2
-        hence False by auto
-        thus ?case by simp
-      next case ev_case_let
-        hence False by auto
-        thus ?case by simp
-      qed simp_all
-  next case (ev_case2 cs l e' ts e t)
-    with ev_case2(2) show ?case
-      proof (induction "Case (Inj l ts e) t cs" e'' rule: evaluate.induct)
-      case ev_case1
-        hence False by auto
-        thus ?case by simp
-      qed simp_all
-  next case (ev_case_let e\<^sub>2 e\<^sub>1 t cs)
-    with ev_case_let(2) show ?case
-      proof (induction "Case (Let e\<^sub>1 e\<^sub>2) t cs" e'' rule: evaluate.induct)
-      case ev_case1
-        hence False by auto
-        thus ?case by simp
-      qed simp_all
-  next case (ev_unfold1 e e' t)
-    with ev_unfold1(3) show ?case
-      proof (induction "Unfold t e" e'' rule: evaluate.induct)
-      case ev_unfold2
-        hence False by auto
-        thus ?case by simp
-      next case ev_unfold_let
-        hence False by auto
-        thus ?case by simp
-      qed simp_all
-  next case (ev_unfold2 t e)
-    thus ?case
-      proof (induction "Unfold t (Fold t e)" e'' rule: evaluate.induct)
-      case ev_unfold1
-        hence False by auto
-        thus ?case by simp
-      qed simp_all
-  next case (ev_unfold_let e\<^sub>2 e\<^sub>1 t)
-    with ev_unfold_let(2) show ?case
-      proof (induction "Unfold e\<^sub>1 (Let t e\<^sub>2)" e'' rule: evaluate.induct)
-      case ev_unfold1
-        hence False by auto
-        thus ?case by simp
-      qed simp_all
-  next case (ev_tyapp1 e e' t)
-    with ev_tyapp1(3) show ?case
-      proof (induction "TyApp e t" e'' rule: evaluate.induct)
-      case ev_tyapp2
-        hence False by auto
-        thus ?case by simp
-      next case ev_tyapp_let
-        hence False by auto
-        thus ?case by simp
-      qed simp_all
-  next case (ev_tyapp2 k e t)
-    thus ?case
-      proof (induction "TyApp (TyAbs k e) t" e'' rule: evaluate.induct)
-      case ev_tyapp1
-        hence False by auto
-        thus ?case by simp
-      qed simp_all
-  next case (ev_tyapp_let e\<^sub>2 e\<^sub>1 t)
-    with ev_tyapp_let(2) show ?case 
-      by (induction "TyApp (Let e\<^sub>1 e\<^sub>2) t" e'' rule: evaluate.induct) auto
-  next case (ev_tylet t e)
-    thus ?case by (induction "TyLet t e" e'' rule: evaluate.induct) simp_all
+theorem determinism [elim]: "e \<Down> v \<Longrightarrow> e \<Down> v' \<Longrightarrow> v = v'"
+  proof (induction e v arbitrary: v' rule: reduce.induct)
+  case (red_var x)
+    thus ?case by (induction "Var x" v' rule: reduce.induct) blast+
+  next case (red_abs t e)
+    thus ?case by (induction "Abs t e" v' rule: reduce.induct) blast+
+  next case (red_app e\<^sub>1 _ _ e\<^sub>2)
+    with red_app(5) show ?case by (induction "App e\<^sub>1 e\<^sub>2" v' rule: reduce.induct) blast+
+  next case (red_app_let e\<^sub>1 _ _ e\<^sub>2)
+    with red_app_let(5) show ?case by (induction "App e\<^sub>1 e\<^sub>2" v' rule: reduce.induct) blast+
+  next case (red_let_0 _ e\<^sub>2 e\<^sub>1)
+    with red_let_0(8) show ?case by (induction "Let e\<^sub>1 e\<^sub>2" v' rule: reduce.induct) blast+
+  next case (red_let_S _ e\<^sub>2 e\<^sub>1)
+    with red_let_S(4) show ?case by (induction "Let e\<^sub>1 e\<^sub>2" v' rule: reduce.induct) metis+
+  next case (red_rec xs)
+    thus ?case by (induction "Rec xs" v' rule: reduce.induct) blast+
+  next case (red_proj _ l _ e)
+    with red_proj(4) show ?case by (induction "Proj e l" v' rule: reduce.induct) fastforce+
+  next case (red_proj_let e _ _ l)
+    with red_proj_let(5) show ?case by (induction "Proj e l" v' rule: reduce.induct) blast+
+  next case (red_inj l ts x)
+    thus ?case by (induction "Inj l ts x" v' rule: reduce.induct) blast+
+  next case (red_case cs l e' e ts x v t)
+    with red_case(6) show ?case 
+      proof (induction "Case e t cs" v' rule: reduce.induct)
+      case (red_case l\<^sub>2 e'\<^sub>2 ts\<^sub>2 x\<^sub>2 v\<^sub>2)
+        from red_case(2, 8) have "l\<^sub>2 = l \<and> ts\<^sub>2 = ts \<and> x\<^sub>2 = x" by blast
+        with red_case(1, 4, 5, 9) show ?case by simp
+      qed blast+
+  next case (red_case_let e e\<^sub>1 e\<^sub>2 t cs v)
+    with red_case_let(5) show ?case
+      proof (induction "Case e t cs" v' rule: reduce.induct)
+      case (red_case_let e\<^sub>1' e\<^sub>2' v')
+        from red_case_let(1, 6) have "e\<^sub>1' = e\<^sub>1 \<and> e\<^sub>2' = e\<^sub>2" by blast
+        with red_case_let(3, 7) show ?case by simp
+      qed blast+
+  next case (red_fold t x)
+    thus ?case by (induction "Fold t x" v' rule: reduce.induct) blast+
+  next case (red_unfold e t)
+    with red_unfold(3) show ?case by (induction "Unfold t e" v' rule: reduce.induct) blast+
+  next case (red_unfold_let e _ _ t)
+    with red_unfold_let(5) show ?case by (induction "Unfold t e" v' rule: reduce.induct) blast+
+  next case (red_tyabs k e)
+    thus ?case by (induction "TyAbs k e" v' rule: reduce.induct) blast+
+  next case (red_tyapp e _ _ t)
+    with red_tyapp(5) show ?case by (induction "TyApp e t" v' rule: reduce.induct) blast+
+  next case (red_tyapp_let e _ _ t)
+    with red_tyapp_let(5) show ?case by (induction "TyApp e t" v' rule: reduce.induct) blast+
+  next case (red_tylet t e)
+    with red_tylet(3) show ?case by (induction "TyLet t e" v' rule: reduce.induct) blast+
   qed
-
-*)
 
 end
