01Expression/03EvaluationContext/ContextEvaluate.thy
@@ -27,29 +27,6 @@ inductive evaluate :: "expr \<Rightarrow> expr \<Rightarrow> bool" (infix "\<lea
 | ev_tyapp_let [simp]: "is_value e\<^sub>2 \<Longrightarrow> TyApp (Let e\<^sub>1 e\<^sub>2) t \<leadsto> Let e\<^sub>1 (TyApp e\<^sub>2 t)" 
 | ev_tylet [simp]: "TyLet t e \<leadsto> subst\<^sub>t\<^sub>e 0 t e" 
 
-lemma canonical_arrow [simp]: "\<Delta>,\<Gamma> \<turnstile> e : Arrow t\<^sub>1 t\<^sub>2 \<Longrightarrow> is_value e \<Longrightarrow> 
-    (\<exists>e'. e = Abs t\<^sub>1 e') \<or> (\<exists>e\<^sub>1 e\<^sub>2. e = Let e\<^sub>1 e\<^sub>2 \<and> is_value e\<^sub>2)"
-  by (induction \<Gamma> e "Arrow t\<^sub>1 t\<^sub>2" rule: typecheck_typecheck_cs.inducts(1)) simp_all
-
-lemma canonical_record [simp]: "\<Delta>,\<Gamma> \<turnstile> e : Record ts \<Longrightarrow> is_value e \<Longrightarrow> 
-    (\<exists>fs. e = Rec fs \<and> \<Delta>,\<Gamma> \<turnstile>\<^sub>x\<^sub>s fs : ts) \<or> (\<exists>e\<^sub>1 e\<^sub>2. e = Let e\<^sub>1 e\<^sub>2 \<and> is_value e\<^sub>2)"
-  by (induction \<Gamma> e "Record ts" rule: typecheck_typecheck_cs.inducts(1)) simp_all
-
-lemma canonical_variant [simp]: "\<Delta>,\<Gamma> \<turnstile> e : Variant ts \<Longrightarrow> is_value e \<Longrightarrow> 
-    (\<exists>l e'. e = Inj l ts e' \<and> l < length ts) \<or> (\<exists>e\<^sub>1 e\<^sub>2. e = Let e\<^sub>1 e\<^sub>2 \<and> is_value e\<^sub>2)"
-  by (induction \<Gamma> e "Variant ts" rule: typecheck_typecheck_cs.inducts(1)) auto
-
-lemma canonical_inductive [simp]: "\<Delta>,\<Gamma> \<turnstile> e : Inductive k t \<Longrightarrow> is_value e \<Longrightarrow> 
-    (\<exists>e'. e = Fold t e') \<or> (\<exists>e\<^sub>1 e\<^sub>2. e = Let e\<^sub>1 e\<^sub>2 \<and> is_value e\<^sub>2)"
-  by (induction \<Gamma> e "Inductive k t" rule: typecheck_typecheck_cs.inducts(1)) auto
-
-lemma canonical_forall [simp]: "\<Delta>,\<Gamma> \<turnstile> e : Forall k t \<Longrightarrow> is_value e \<Longrightarrow> 
-    (\<exists>e'. e = TyAbs k e') \<or> (\<exists>e\<^sub>1 e\<^sub>2. e = Let e\<^sub>1 e\<^sub>2 \<and> is_value e\<^sub>2)"
-  by (induction \<Gamma> e "Forall k t" rule: typecheck_typecheck_cs.inducts(1)) auto
-
-lemma lookup_in_tc [simp]: "\<Delta>,\<Gamma> \<turnstile>\<^sub>x\<^sub>s fs : ts \<Longrightarrow> lookup ts l = Some t \<Longrightarrow> \<exists>e. lookup fs l = Some e"
-  by (induction fs l arbitrary: ts rule: lookup.induct) auto
-
 lemma progress': "\<Delta>,\<Gamma> \<turnstile> e : t \<Longrightarrow> 
   is_value e \<or> (\<exists>e'. e \<leadsto> e') \<or> (\<exists>x < length \<Gamma>. head_var e = Some x)"
     and "\<Delta>,\<Gamma> \<turnstile>\<^sub>c cs : ts \<rightarrow> t \<Longrightarrow> l < length ts \<Longrightarrow> \<exists>c. lookup cs l = Some c"
